\documentclass{article}
\usepackage{amsmath}

\begin{document}

\subsection{Sequence operations}

$$ (a+b)_n = a_n + b_n \qquad ab_n = \sum_{k=0}^{n} a_{n-k} b_k $$

\subsection{The signature function and the signature left near-ring}

$$F_{d}(0) = 1 \qquad  F_{d}(n) = \sum_{k=1}^{n} F_{d}(n-k) \cdot d_{k-1} \qquad F_{d}^{-1}(n) = d_{n+1} - \sum_{k=1}^{n} d_{n-k} \cdot F_{d}^{-1}(k-1)$$

$$a \oplus b = F^{-1} (F_a \otimes F_b) = a + b - abx \qquad a \circ b = \sum_{k=0}^{n} a^{k+1} x^k b_k$$

\subsection{The general signature function and prismatic convolution}

\noindent Let $T$ and $M$ be matrices with $N$ and $K$ dimensions respectively.

$$F_{T} (n) = \sum_{r_0 + r_1 + ... + r_{N-1} = n} T(r_0, r_1, ..., r_{N-1})$$

$$T \times M (r_0, r_1, ... r_{N + K - 2}) = \left( T(r_0, r_1, ..., r_{N - 2}) \otimes M (r_{N-1}, r_N, ..., r_{N + K - 3}) \right) (r_{N + K - 2})$$

$$F_{T \times M} = F_T \otimes F_M$$

\noindent If $T$ and $M$ are one-beginning, we also have:

$$F_{T \times M}^{-1} = F_T^{-1} \oplus F_M^{-1}$$

\subsection{General signature convolution}

\noindent Let $T$ be given by the following prism:

$$T =  T_{g_0} \times ... \times T_{g_{N-2}}$$

\noindent Where $T_g$ is a power triangle whose signature is $g$.

$$F_{T \circ S}(n) = \sum_{r_0 + ... + r_{N-1} = n} T(r_0, ... , r_{N-1}) \cdot \prod_{k=0}^{N-2} F_{S_k} (r_k) $$

\subsection{The signature dot product}

$$T \circ S = \bigoplus_{k=0}^{N-2} g_k \circ S_k$$

\end{document}